theories/region_invariants_static.v
@@ -5,10 +5,13 @@ Require Import stdpp.countable.
 Import uPred.
 
 Section heap.
-  Context `{heapG Σ, memG Σ, regG Σ, STSG Σ,
-            MonRef: MonRefG (leibnizO _) CapR_rtc Σ}.
+  Context {Σ:gFunctors} {memg:memG Σ} {regg:regG Σ}
+          {stsg : STSG Addr region_type Σ} {heapg : heapG Σ}
+          `{MonRef: MonRefG (leibnizO _) CapR_rtc Σ}.
+
   Notation STS := (leibnizO (STS_states * STS_rels)).
-  Notation WORLD := (prodO STS STS).
+  Notation STS_STD := (leibnizO (STS_std_states Addr region_type)).
+  Notation WORLD := (prodO STS_STD STS). 
   Implicit Types W : WORLD.
 
   (* This file provides three main lemmas:
@@ -156,12 +159,12 @@ Section heap.
 
   (* A collection of sts_state_std *)
   Definition sts_state_std_many {V} (m: gmap Addr V) (ρ: region_type) :=
-    ([∗ map] a↦_ ∈ m, sts_state_std (encode a) ρ)%I.
+    ([∗ map] a↦_ ∈ m, sts_state_std a ρ)%I.
 
   (* Bulk update of the state of a [sts_state_std_many] *)
   Lemma region_update_multiple_states W (m : gmap Addr (Perm * Word)) st st' :
-    sts_full_world sts_std W ∗ sts_state_std_many m st
-    ==∗ sts_full_world sts_std (std_update_multiple W (elements (dom (gset Addr) m)) st')
+    sts_full_world W ∗ sts_state_std_many m st
+    ==∗ sts_full_world (std_update_multiple W (elements (dom (gset Addr) m)) st')
     ∗ sts_state_std_many m st'.
   Proof.
     iIntros "[Hfull Hstate]".
@@ -169,19 +172,18 @@ Section heap.
     - rewrite /sts_state_std_many dom_empty_L elements_empty big_sepM_empty big_sepM_empty /=.
       iModIntro. iFrame.
     - iDestruct (big_sepM_insert with "Hstate") as "[Hx Hstate]";auto.
+      iDestruct (sts_full_state_std with "Hfull Hx") as %Hstate. 
       iMod ("IH" with "Hfull Hstate") as "[Hfull Hstate]". iClear "IH".
       iMod (sts_update_std _ _ _ st' with "Hfull Hx") as "[Hfull Hx]".
       rewrite dom_insert_L.
       erewrite (std_update_multiple_permutation _ (elements (_ ∪ _))).
-      2: { rewrite elements_union_singleton // not_elem_of_dom //. }
-      iDestruct (sts_full_world_std with "Hfull") as %Hstd.
-      iAssert (⌜is_Some ((std_update_multiple W (elements (dom (gset Addr) m)) st').1.2 !! (encode x))⌝%I)
+      2: { rewrite elements_union_singleton // not_elem_of_dom //. }      
+      iAssert (⌜is_Some ((std_update_multiple W (elements (dom (gset Addr) m)) st').1 !! x)⌝%I)
         as %Hsome.
-      { rewrite /sts_full_world /sts_full_std /=. iDestruct "Hfull" as "[ [#Hdom _] _]".
-        iDestruct "Hdom" as %Hdom. iPureIntro.
-        rewrite elem_of_gmap_dom. rewrite dom_insert_L in Hdom. set_solver. }
-      pose proof (Hstd _ Hsome) as Hstdx.
-      apply insert_id in Hstdx. rewrite /std_rel /= in Hstdx. rewrite -Hstdx. iFrame.
+      { rewrite /sts_full_world /sts_full_std /=. 
+        iPureIntro. apply std_sta_update_multiple_is_Some.
+        eauto. }
+      iFrame.
       iModIntro. iApply big_sepM_insert;auto. iFrame.
   Qed.
 
@@ -195,7 +197,7 @@ Section heap.
     m !! l = Some (p, v) →
     region_map_def M Mρ W -∗
     region_map_def (delete l M) Mρ W ∗
-    l ↦ₐ[p] v ∗ sts_state_std (encode l) (Static m).
+    l ↦ₐ[p] v ∗ sts_state_std l (Static m).
   Proof.
     intros Hdom HMl HMρ Hm.
     iIntros "Hr". destruct HMl as [? ?].
@@ -215,10 +217,10 @@ Section heap.
     (forall a', a' ∈ dom (gset Addr) m → Mρ !! a' = Some (Static m_all)) →
     dom (gset Addr) Mρ = dom (gset Addr) M →
     region_map_def M Mρ W
-    ∗ sts_full_world sts_std W
+    ∗ sts_full_world W
     -∗
     region_map_def (M ∖∖ m) Mρ W
-    ∗ sts_full_world sts_std W
+    ∗ sts_full_world W
     ∗ static_resources m
     ∗ sts_state_std_many m (Static m_all).
   Proof.
@@ -253,10 +255,10 @@ Section heap.
     (forall a', a' ∈ dom (gset Addr) m → Mρ !! a' = Some (Static m)) →
     dom (gset Addr) Mρ = dom (gset Addr) M →
     region_map_def M Mρ W
-    ∗ sts_full_world sts_std W
+    ∗ sts_full_world W
     -∗
     region_map_def (M ∖∖ m) (Mρ ∖∖ m) W
-    ∗ sts_full_world sts_std W
+    ∗ sts_full_world W
     ∗ sts_state_std_many m (Static m)
     ∗ static_resources m.
   Proof.
@@ -279,30 +281,29 @@ Section heap.
   Qed.
 
   Lemma region_map_has_static_addr M Mρ W (l: Addr) m :
-    (std_sta W) !! (encode l) = Some (encode (Static m)) →
-    dom_equal (std_sta W) M →
-    region_map_def M Mρ W ∗ sts_full_world sts_std W -∗
+    (std W) !! l = Some (Static m) →
+    dom (gset Addr) (std W) = dom (gset Addr) M →
+    region_map_def M Mρ W ∗ sts_full_world W -∗
     ⌜(forall a', a' ∈ dom (gset Addr) m → Mρ !! a' = Some (Static m))⌝ ∗
     ⌜l ∈ dom (gset Addr) m⌝.
   Proof.
-    iIntros (HWl Hdom) "(Hr & Hsts)". unfold dom_equal in Hdom.
-    specialize (Hdom (encode l)) as [Hdom _].
-    feed destruct Hdom as (a & ?%encode_injective & (? & ?)); eauto.
-    subst a.
+    iIntros (HWl Hdom) "(Hr & Hsts)". 
+    assert (is_Some (M !! l)) as [ρ Hρ].
+    { apply elem_of_gmap_dom. rewrite -Hdom. apply elem_of_gmap_dom. eauto. }
     iDestruct (big_sepM_lookup _ _ l with "Hr") as "Hl"; eauto.
-    iDestruct "Hl" as (ρ Hρ) "(Hst & Hρ)".
+    iDestruct "Hl" as (ρ' Hρ') "(Hst & Hρ)".
     iDestruct (sts_full_state_std with "Hsts Hst") as %HH.
-    rewrite HWl in HH. apply Some_eq_inj, encode_injective in HH. subst ρ.
+    rewrite HWl in HH. apply Some_eq_inj in HH. subst ρ'.
     iDestruct "Hρ" as (? ? ?) "(? & ? & ? & Hρ)". 
     iDestruct "Hρ" as (? ? ?) "(? & ? & %)". intros. iPureIntro. split; eauto.
     rewrite -elem_of_gmap_dom; eauto.
   Qed.
 
   Lemma region_open_static W (m: gmap Addr (Perm * Word)) (l: Addr) :
-    (std_sta W) !! (encode l) = Some (encode (Static m)) →
-    region W ∗ sts_full_world sts_std W -∗
+    (std W) !! l = Some (Static m) →
+    region W ∗ sts_full_world W -∗
     open_region_many (elements (dom (gset Addr) m)) W
-    ∗ sts_full_world sts_std W
+    ∗ sts_full_world W
     ∗ sts_state_std_many m (Static m)
     ∗ static_resources m
     ∗ ⌜l ∈ dom (gset Addr) m⌝.
@@ -323,40 +324,35 @@ Section heap.
   (* ---------------------- Turn a static region into a temporary one ---------------- *)
 
   Lemma related_sts_pub_world_static_to_temporary (l: list Addr) m W:
-    rel_is_std W →
-    Forall (λ (a:Addr), (std_sta W) !! (encode a) = Some (encode (Static m))) l →
+    Forall (λ (a:Addr), (std W) !! a = Some (Static m)) l →
     related_sts_pub_world W (std_update_multiple W l Temporary).
   Proof.
-    intros Hstd Hforall.
+    intros Hforall.
     induction l.
-    - split; apply related_sts_pub_refl.
+    - apply related_sts_pub_refl_world.
     - rewrite Forall_cons in Hforall *; move=>[Ha Hforall].
       eapply related_sts_pub_trans_world;[by apply IHl|].
       cbn. set W' := std_update_multiple W l Temporary.
       rewrite /std_update /related_sts_pub_world /=. split.
       2: { apply related_sts_pub_refl. }
-      unfold related_sts_pub. rewrite !dom_insert_L.
+      unfold related_sts_std_pub. rewrite dom_insert_L.
       repeat split_and; [set_solver ..|].
-      intros i r1 r2 r1' r2' Hr Hr'.
-      apply std_update_multiple_rel_is_std with (l:=l) (ρ:=Temporary) in Hstd.
-      rewrite -/W' in Hstd.
-      feed pose proof (Hstd i) as Hstdi; eauto. rewrite /rel_is_std_i /= in Hstdi.
-      unfold std_sta, std_rel in *. simplify_eq.
-      destruct (decide (i = encode a)).
-      { subst i. rewrite lookup_insert in Hr'. simplify_eq. do 2 split; eauto.
-        intros x y Hx Hy. simplify_map_eq.
+      intros i x y Hx Hy.
+      (* apply std_update_multiple_rel_is_std with (l:=l) (ρ:=Temporary) in Hstd. *)
+      (* rewrite -/W' in Hstd. *)
+      (* feed pose proof (Hstd i) as Hstdi; eauto. rewrite /rel_is_std_i /= in Hstdi. *)
+      destruct (decide (i = a)).
+      { subst i. simplify_map_eq. 
         destruct (decide (a ∈ l)).
-        { rewrite std_sta_update_multiple_lookup_in // in Hx. simplify_eq. reflexivity. }
-        rewrite std_sta_update_multiple_lookup_same /std_sta // in Hx. simplify_eq.
-        eapply rtc_once, convert_rel_of_rel. constructor. }
-      { rewrite lookup_insert_ne // in Hr'. rewrite Hr in Hr'. simplify_eq.
-        do 2 split; eauto. intros x y Hx Hy. rewrite lookup_insert_ne // in Hy.
+        { rewrite std_sta_update_multiple_lookup_in_i // in Hx. simplify_eq. reflexivity. }
+        rewrite std_sta_update_multiple_lookup_same_i /std // in Hx. simplify_eq.
+        eapply rtc_once. rewrite Ha in Hx;inversion Hx. constructor. }
+      {  rewrite lookup_insert_ne // in Hy.
         rewrite Hx in Hy; simplify_eq. reflexivity. }
   Qed.
 
   Lemma open_region_world_static_to_temporary l m W :
-    rel_is_std W →
-    Forall (λ (a:Addr), (std_sta W) !! (encode a) = Some (encode (Static m))) l →
+    Forall (λ (a:Addr), (std W) !! a = Some (Static m)) l →
     open_region_many l W
     -∗
     open_region_many l (std_update_multiple W l Temporary).
@@ -365,8 +361,7 @@ Section heap.
     { apply elem_of_equiv_L. intro.
       rewrite -std_update_multiple_dom_equal; auto.
       intros i Hi. apply elem_of_gmap_dom.
-      apply elem_of_list_fmap in Hi as [y [Heq Hy] ]. subst. 
-      eexists. eapply Forall_forall in H4; eauto. }
+      eexists. eapply Forall_forall in H; eauto. }
     { eapply related_sts_pub_world_static_to_temporary; eauto. }
   Qed.
 
@@ -375,9 +370,9 @@ Section heap.
     ∗ ([∗ map] a↦pv ∈ m, ∃ p _v φ, ⌜forall Wv, Persistent (φ Wv)⌝ ∗
         ⌜pv = (p, _v)⌝ ∗ temp_resources W φ a p ∗ rel a p φ)
     ∗ sts_state_std_many m Temporary
-    ∗ sts_full_world sts_std W
+    ∗ sts_full_world W
     -∗
-    region W ∗ sts_full_world sts_std W.
+    region W ∗ sts_full_world W.
   Proof.
     pattern m. revert m. eapply map_ind.
     - iIntros "(Hor & ? & ? & Hsts)". rewrite dom_empty_L elements_empty.
@@ -408,10 +403,10 @@ Section heap.
   Qed.
 
   Lemma sts_full_state_std_many {V} (m: gmap Addr V) (ρ:region_type) W:
-    sts_full_world sts_std W
+    sts_full_world W
     ∗ sts_state_std_many m ρ
     -∗
-    ⌜Forall (λ (a:Addr), std_sta W !! encode a = Some (encode ρ)) (elements (dom (gset Addr) m))⌝.
+    ⌜Forall (λ (a:Addr), std W !! a = Some ρ) (elements (dom (gset Addr) m))⌝.
   Proof.
     pattern m. revert m. apply map_ind.
     - iIntros. iPureIntro. rewrite dom_empty elements_empty //.
@@ -425,16 +420,15 @@ Section heap.
 
   Lemma region_close_static_to_temporary (m: gmap Addr (Perm * Word)) W :
     open_region_many (elements (dom (gset Addr) m)) W
-    ∗ sts_full_world sts_std W
+    ∗ sts_full_world W
     ∗ ([∗ map] a↦pv ∈ m, ∃ p _v φ, ⌜forall Wv, Persistent (φ Wv)⌝ ∗
          ⌜pv = (p, _v)⌝ ∗ temp_resources W φ a p ∗ rel a p φ)
     ∗ sts_state_std_many m (Static m)
     ==∗
-    sts_full_world sts_std (std_update_multiple W (elements (dom (gset Addr) m)) Temporary)
+    sts_full_world (std_update_multiple W (elements (dom (gset Addr) m)) Temporary)
     ∗ region (std_update_multiple W (elements (dom (gset Addr) m)) Temporary).
   Proof.
     iIntros "(HR & Hsts & Hres & Hst)".
-    iDestruct (sts_full_world_std with "Hsts") as %?.
     iDestruct (sts_full_state_std_many with "[Hsts Hst]") as %?. by iFrame.
     iDestruct (region_update_multiple_states with "[$Hsts $Hst]") as ">[Hsts Hst]".
     iModIntro.
@@ -454,16 +448,15 @@ Section heap.
   (* In this version the user is only required to show that the resources are valid in the updated world *)
   Lemma region_close_static_to_temporary_alt (m: gmap Addr (Perm * Word)) W :
     open_region_many (elements (dom (gset Addr) m)) W
-    ∗ sts_full_world sts_std W
+    ∗ sts_full_world W
     ∗ ([∗ map] a↦pv ∈ m, ∃ p _v φ, ⌜forall Wv, Persistent (φ Wv)⌝ ∗
          ⌜pv = (p, _v)⌝ ∗ temp_resources (std_update_multiple W (elements (dom (gset Addr) m)) Temporary) φ a p ∗ rel a p φ)
     ∗ sts_state_std_many m (Static m)
     ==∗
-    sts_full_world sts_std (std_update_multiple W (elements (dom (gset Addr) m)) Temporary)
+    sts_full_world (std_update_multiple W (elements (dom (gset Addr) m)) Temporary)
     ∗ region (std_update_multiple W (elements (dom (gset Addr) m)) Temporary).
   Proof.
     iIntros "(HR & Hsts & Hres & Hst)".
-    iDestruct (sts_full_world_std with "Hsts") as %?.
     iDestruct (sts_full_state_std_many with "[Hsts Hst]") as %?. by iFrame.
     iDestruct (region_update_multiple_states with "[$Hsts $Hst]") as ">[Hsts Hst]".
     iModIntro.
@@ -475,64 +468,43 @@ Section heap.
   (* ------------------ Allocate a Static region from a Revoked one ------------------ *)
 
   Lemma related_sts_pub_world_static W W' m i :
-    rel_is_std_i W i ->
-    (std_sta W !! i) = Some (countable.encode (Static m)) ->
+    (std W !! i) = Some (Static m) ->
     related_sts_pub_world W W' ->
-    (std_sta W' !! i) = Some (countable.encode (Static m)) ∨ (std_sta W' !! i) = Some (countable.encode Temporary).
+    (std W' !! i) = Some (Static m) ∨ (std W' !! i) = Some Temporary.
   Proof.
-    intros Hrel Hsta [ [Hdom1 [Hdom2 Hrelated_std] ] _].
-    assert (is_Some (std_rel W' !! i)) as [ [r1' r2'] Hr']. 
-    { apply elem_of_gmap_dom. assert (i ∈ dom (gset positive) (std_rel W));[apply elem_of_gmap_dom;eauto|]. set_solver. }
-    eapply Hrelated_std in Hr' as [Heq1 [Heq2 Hrelated] ];[subst|eauto]. 
-    assert (is_Some (std_sta W' !! i)) as [y Hy]. 
-    { apply elem_of_gmap_dom. assert (i ∈ dom (gset positive) (std_sta W));[apply elem_of_gmap_dom;eauto|]. set_solver. }
-    eapply Hrelated in Hsta;[|eauto].
+    intros Hsta [ [Hdom1 Hrelated_std] _].
+    assert (is_Some (std W' !! i)) as [y Hy]. 
+    { apply elem_of_gmap_dom. assert (i ∈ dom (gset Addr) (std W));[apply elem_of_gmap_dom;eauto|]. set_solver. }
+    eapply Hrelated_std in Hsta;[|eauto].
     eapply std_rel_pub_rtc_Static in Hsta;[|eauto].
     destruct Hsta as [-> | ->];auto. 
   Qed. 
     
   Lemma related_sts_priv_world_static W l (m' : gmap Addr (Perm * Word)) :
-    rel_is_std W -> 
-    Forall (λ a : Addr, (std_sta W) !! (encode a) = Some (encode Revoked)) l →
+    Forall (λ a : Addr, (std W) !! a = Some Revoked) l →
     related_sts_priv_world W (std_update_multiple W l (Static m')).
   Proof.
-    intros Hstd Hforall.
+    intros Hforall.
     induction l. 
-    - split;apply related_sts_priv_refl. 
+    - apply related_sts_priv_refl_world. 
     - eapply related_sts_priv_trans_world;[apply IHl|].
       + apply Forall_cons_1 in Hforall as [_ Hforall]. auto. 
       + split;[|rewrite std_update_multiple_loc_rel;apply related_sts_priv_refl].
-        split;[|split].
+        split. 
         ++ rewrite /std_update dom_insert_L. set_solver.
-        ++ rewrite /std_update dom_insert_L. set_solver.
-        ++ intros j r1 r2 r1' r2' Hr Hr'.
-           rewrite /std_update in Hr'. simpl in *.
-           apply std_update_multiple_rel_is_std with (l:=l) (ρ:=Static m') in Hstd.
-           assert (is_Some (std_rel (std_update_multiple W l (Static m')) !! j)) as Hsome.
-           eauto. apply Hstd in Hsome.
-           destruct (decide (encode a = j)).
-           +++ subst. rewrite lookup_insert in Hr'.
-               rewrite Hsome in Hr. inversion Hr'; inversion Hr; subst.
-               repeat split;auto.
-               intros x0 y Hx0 Hy. rewrite lookup_insert in Hy. inversion Hy; subst.
+        ++ intros j x0 y Hx0 Hy.
+           destruct (decide (a = j)).
+           +++ subst. rewrite lookup_insert in Hy. inversion Hy; subst.
                apply Forall_cons_1 in Hforall as [Hi _].
-               destruct (decide (a ∈ l)).
-               { rewrite std_sta_update_multiple_lookup_in in Hx0; auto. inversion Hx0. left. }
-               rewrite std_sta_update_multiple_lookup_same in Hx0; auto.
-               rewrite /revoke /std_sta /= in Hi. (* apply anti_revoke_lookup_Revoked in Hi as [Hrev | Htemp]. *)
-               (* * rewrite Hrev in Hx0. inversion Hx0; subst. *)
+               destruct (decide (j ∈ l)).
+               { rewrite std_sta_update_multiple_lookup_in_i in Hx0; auto. inversion Hx0. left. }
+               rewrite std_sta_update_multiple_lookup_same_i in Hx0; auto.
+               rewrite /revoke /std /= in Hi.
                rewrite Hi in Hx0. inversion Hx0; subst. 
-               right with (encode Temporary).
-               { left. exists Revoked,Temporary. repeat split;auto. constructor. }
-               right with (encode (Static m'));[|left]. right. exists Temporary,(Static m'). repeat split;auto.
-               constructor. 
-               (* * rewrite Htemp in Hx0; inversion Hx0; auto. *)
-               (*   right with (encode (Static m'));[|left]. right. exists Temporary,(Static m'). repeat split;auto. *)
-               (*   constructor. *)
-           +++ rewrite lookup_insert_ne in Hr'; auto. rewrite Hsome in Hr'. rewrite Hsome in Hr.
-               inversion Hr'; inversion Hr. subst. repeat split;auto.
-               intros x y Hx Hy.
-               rewrite lookup_insert_ne in Hy;auto. rewrite Hx in Hy; inversion Hy; subst; left.
+               right with Temporary.
+               { left. constructor. }
+               right with (Static m');[|left]. right. constructor. 
+           +++ rewrite /= lookup_insert_ne in Hy;auto. rewrite Hx0 in Hy; inversion Hy; subst; left.
   Qed.
 
   Lemma std_update_multiple_dom_equal_eq W M (m: gmap Addr (Perm * Word)) ρ :
